ch2.6 ex1.v: do some excercises

ch02/ex1.v
@@ -1,4 +1,6 @@
-Require Import Arith.
+Require Import Bool Arith ZArith List.
+
+Import ListNotations.
 
 (* EXAMPLES *) 
 (* The following function takes two arguments a and b
@@ -17,15 +19,18 @@ Definition add_pair_components (p : nat * nat) :=
 
 (* 1/ Define a function that takes two numbers as arguments and returns
   the sum of the squares of these numbers. *)
+Definition sumsq (a b : nat) := a * a + b * b.
 
 (* 2/ Define a function that takes 5 arguments a b c d e, which are all
    numbers and returns the sum of all these numbers. *)
+Definition sum5 (a b c d e : nat) := a + b + c + d + e.
 
 (* 3/ Define a function named add5 that takes a number as argument and returns
    this number plus 5. *)
+Definition add5 := Nat.add 5.
 
 (* The following should return 8 *)
-(* Compute add5 3.*)
+Compute add5 3.
 
 (* The following commands make it possible to find pre-defined functions
 Search nat.
@@ -35,6 +40,23 @@ Search bool.
 (* 4/ Write a function swap of type list nat -> list nat such that
   swap (a::b::l) = (b::a::l)  and
   swap l' = l' if l' has less than 2 elements. *)
+Definition swap (ns : list nat) : list nat
+  := match ns with
+     | [] | [_] => ns
+     | n1 :: n2 :: ns' => n2 :: n1 :: ns'
+     end.
+
+Theorem swap_long (a b : nat) (l : list nat) : swap (a::b::l) = (b::a::l).
+Proof. reflexivity. Qed.
+
+Theorem swap_short (ns : list nat) : length ns < 2 -> swap ns = ns.
+Proof.
+  intro H.
+  destruct ns; try reflexivity.
+  destruct ns; try reflexivity.
+  repeat apply lt_S_n in H.
+  now apply Nat.nlt_0_r in H.
+Qed.
 
 (* 5/ Write a function proc2 of type list nat -> nat, such that
    proc2 (a::b::l) = (b + 3) and
@@ -43,21 +65,105 @@ Search bool.
    In other words, proc2 only processes the 2nd argument of the list and
    returns that number plus 3.  If there is no second argument to the list,
    proc2 returns 0.  *)
+Definition proc2 (ns : list nat) : nat
+  := match ns with
+     | [] | [_] => 0
+     | n1 :: n2 :: _  => n2 + 3
+     end.
 
 (* 6/ Write a function ms of type list nat -> list nat such that
       ms (a::b::...::nil) = a+2::b+2::...::nil
       For instance
-      ms (2::3::5::nil) = (4::5::7::nil) *) 
+      ms (2::3::5::nil) = (4::5::7::nil) *)
+Fixpoint ms (ns : list nat) : list nat
+  := match ns with
+     | [] => []
+     | n :: ns' => (n + 2) :: (ms ns')
+     end.
+
+Example ms_ex : ms (2::3::5::nil) = (4::5::7::nil).
+Proof. reflexivity. Qed.
 
 (* 7/ Write a function sorted of type list nat -> bool, such that
     sorted l = true exactly when the natural numbers in
    l are in increasing order. *)
+Definition sorted (ns : list nat) : bool
+  := let fix iter (n : nat) (ns : list nat)
+         := match ns with
+            | [] => true
+            | n' :: ns' => (n <=? n') && iter n' ns'
+            end
+     in match ns with
+        | [] => true
+        | n :: ns' => iter n ns'
+        end.
 
-(* 8/ Write a function p2 of type nat -> nat such that 
+Example sorted_ex : sorted [1; 3; 3; 5] = true.
+Proof. reflexivity. Qed.
+
+Example sorted_ex2 : sorted [1; 3; 2; 3; 5] = false.
+Proof. reflexivity. Qed.
+
+Inductive sorted_p  : list nat -> Prop
+  := sorted0 : sorted_p []
+   | sorted1 (n : nat) : sorted_p [n]
+   | sorted_n (n0 n1 : nat) (ns : list nat) :
+       n0 <= n1
+       -> sorted_p (n1 :: ns)
+       -> sorted_p (n0 :: n1 :: ns).
+
+Example sorted_p_ex : sorted_p [1; 3; 3; 5].
+Proof. auto using sorted_p with arith. Qed.
+
+Example sorted_p_ex2 : ~ sorted_p [1; 3; 2; 3; 5].
+Proof.
+  intro H. inversion H. inversion H4.
+  now apply Nat.nle_succ_diag_l in H7.
+Qed.
+
+Theorem iff_true_r (A : Prop) : A -> (A <-> True).
+Proof. firstorder. Qed.
+
+Theorem iff_true_l (A : Prop) : A -> (True <-> A).
+Proof. firstorder. Qed.
+
+Theorem proven_iff (A B : Prop) : A -> B -> (A <-> B).
+Proof. firstorder. Qed.
+
+Theorem sorted_correct (ns : list nat) : sorted ns = true <-> sorted_p ns.
+Proof.
+  induction ns as [| n0 ns0 IH]; try destruct ns0 as [| n1 ns1];
+    try ( apply proven_iff; try reflexivity; constructor ).
+  split; intro H; inversion H.
+  - apply andb_prop in H1 as [H1 H2].
+    apply Nat.leb_le in H1 as H1'.
+    apply sorted_n; try assumption.
+    apply IH. assumption.
+  - subst n2 n3 ns. apply Nat.leb_le in H2 as H2'.
+    assert (sorted (n1 :: ns1) = true) as Hs.
+    { apply IH. assumption. }
+    simpl. apply andb_true_intro; split; assumption.
+Qed.
+
+(* 8/ Write a function p2 of type nat -> nat such that
     p2 n = 2 ^ n *)
+Fixpoint p2 (n : nat) : nat
+  := match n with
+     | O => 1
+     | S n' => 2 * (p2 n')
+     end.
+
+Example p2_ex : p2 3 = 8.
+Proof. reflexivity. Qed.
+
+Theorem p2_correct (n : nat) : Nat.pow 2 n = p2 n.
+Proof.
+  induction n as [| n' IH]; try reflexivity.
+  simpl. rewrite <- IH. ring.
+Qed.
 
 (* 9/ Write a function salt of type nat -> nat -> nat such that
-   salt x n = x ^ n - x^ (n+1) + x^(n-2) .... + 1 or -1, if x <> 0,
+   salt x n = x^n - x^(n-1) + x^(n-2) .... + 1 or -1, if x <> 0,
    depending on the parity of n, thus
    salt x 3 = x^3 - x^2 + x - 1
    salt x 4 = x^4 - x^3 + x^2 - x + 1
@@ -65,17 +171,16 @@ Search bool.
 
    You may have to define auxiliary functions. *)
 
-
 (* 10/  Consider the following definition *)
 
 Inductive btree : Type :=
-|  leaf 
+|  leaf
 |  bnode (n:nat)(t1 t2: btree).
 
 (* write a function that list the labels of a tree by infix order *)
-(** you may use the concatenation function app on lists 
+(** you may use the concatenation function app on lists
   (also written l1 ++ l2 ) *)
 
 
-(* write a boolean function that checks whether a tree is a binary 
+(* write a boolean function that checks whether a tree is a binary
 search tree *)
